

# Examples and Problems in Analysis

TRISCT

## Contents

### 1 Equalities

#### 1.1 Common Taylor Series

1.  $e^x = 1 + x + \frac{x^2}{2} + \cdots + \frac{x^n}{n!} + \cdots \quad (-\infty < x < +\infty)$
2.  $\sin x = x - \frac{x^3}{3!} + \frac{x^5}{5!} + \cdots + (-1)^{n-1} \frac{x^{2n-1}}{(2n-1)!} + \cdots \quad (-\infty < x < +\infty)$
3.  $\cos x = 1 - \frac{x^2}{2!} + \frac{x^4}{4!} + \cdots + (-1)^n \frac{x^{2n}}{(2n)!} + \cdots \quad (-\infty < x < +\infty)$
4.  $(1+x)^\alpha = 1 + \alpha x + \frac{\alpha(\alpha-1)}{2!} x^2 + \cdots + \frac{\alpha(\alpha-1)\cdots(\alpha-n+1)}{n!} x^n + \cdots \quad (-1 < x < 1)$
5.  $\ln(1+x) = x - \frac{x^2}{2} + \frac{x^3}{3} + \cdots + (-1)^{n-1} \frac{x^n}{n} + \cdots \quad (-1 < x \leq x)$
6.  $\arctan x = x - \frac{x^3}{3} + \frac{x^5}{5} + \cdots + (-1)^{n-1} \frac{x^{2n-1}}{2n-1} + \cdots \quad (-1 \leq x \leq 1)$
7.  $\arcsin x = x + \frac{x^3}{6} + \frac{3x^5}{40} + \cdots + \frac{(2n-1)!!x^{2n+1}}{(2n)!!(2n+1)} + \cdots \quad (-1 \leq x \leq 1)$
8.  $\frac{1}{1+x} = (1+x)^{-1} = 1 - x + x^2 - \cdots + (-1)^n x^n + \cdots \quad (-1 < x < 1)$
9.  $\frac{1}{(1+x)^2} = (1+x)^{-2} = 1 - 2x + 3x^2 - \cdots + (-1)^n (n+1)x^n + \cdots \quad (-1 < x < 1)$
10.  $\sqrt{1+x} = (1+x)^{\frac{1}{2}} = 1 + \frac{1}{2}x - \frac{1}{8}x^2 + \cdots + (-1)^{n-1} \frac{(2n-3)!!}{(2n)!!} x^n + \cdots \quad (-1 \leq x \leq 1)$
11.  $\frac{1}{\sqrt{1+x}} = (1+x)^{-\frac{1}{2}} = 1 - \frac{1}{2}x + \frac{3}{8}x^2 - \cdots + (-1)^n \frac{(2n-1)!!}{(2n)!!} x^n + \cdots \quad (-1 < x \leq 1)$

## 1.2 Common Infinite Products

$$1. \sin x = x \prod_{n=1}^{\infty} \left(1 - \frac{x^2}{n^2\pi^2}\right) \quad (-\infty < x < +\infty)$$

$$2. \cos x = \prod_{n=1}^{\infty} \left(1 - \frac{4x^2}{(2n-1)^2\pi^2}\right) \quad (-\infty < x < +\infty)$$

$$3. \frac{\sin x}{x} = \prod_{n=1}^{\infty} \cos \frac{x}{2^n} \quad (x \neq 0)$$

$$4. \prod_{n=0}^{\infty} (1 + x^{2^n}) = \frac{1}{1-x} \quad (-1 < x < 1)$$

## 1.3 Telescoping (1): $\sum_{n=1}^N \cos nx$ and $\sum_{n=1}^N \sin nx$

$$\sum_{n=1}^N \cos nx = \frac{\sin \left(N + \frac{1}{2}\right) x - \sin \frac{x}{2}}{2 \sin \frac{x}{2}} \quad (x \neq 2k\pi)$$

$$\sum_{n=1}^N \sin nx = \frac{\cos \left(N + \frac{1}{2}\right) x - \cos \frac{x}{2}}{-2 \sin \frac{x}{2}} \quad (x \neq 2k\pi)$$

**Note 1.1.** *These are obtained from*

$$\sin \left(n + \frac{1}{2}\right) x - \sin \left(n - \frac{1}{2}\right) x = 2 \sin \frac{x}{2} \cos nx$$

$$\cos \left(n + \frac{1}{2}\right) x - \cos \left(n - \frac{1}{2}\right) x = -2 \sin \frac{x}{2} \sin nx$$

## 1.4 Telescoping (2): $\prod_{n=1}^N \cos \frac{x}{2^n}$

$$\prod_{n=1}^N \cos \frac{x}{2^n} = \frac{1}{2^N} \cdot \frac{\sin x}{\sin \frac{x}{2^N}} \quad (x \neq 0)$$

$$\prod_{n=1}^{\infty} \cos \frac{x}{2^n} = \frac{\sin x}{x} \quad (x \neq 0)$$

**1.5 Telescoping (3):**  $\sum_{n=1}^N \frac{nx}{(1+x)(1+2x)\cdots(1+nx)}$

$$\begin{aligned} & \sum_{n=1}^N \frac{nx}{(1+x)(1+2x)\cdots(1+nx)} \\ &= \sum_{n=1}^N \left( \frac{1}{(1+x)(1+2x)\cdots(1+(n-1)x)} - \frac{1}{(1+x)(1+2x)\cdots(1+nx)} \right) \\ &= 1 - \frac{1}{(1+x)(1+2x)\cdots(1+Nx)} \end{aligned}$$

**1.6 Formula (1):**  $\sqrt{2 + \sqrt{2 + \cdots + \sqrt{2}}} = 2 \cos \frac{\pi}{2^{n+1}}$

Use

$$\cos \frac{x}{2} = \sqrt{\frac{1}{2} + \frac{1}{2} \cos x}$$

**1.7 Order Estimate (1):**  $\frac{p(p+1)\cdots(p+n-1)}{n!}$

$p \neq 0$  is not a negative integer, then

$$\frac{p(p+1)\cdots(p+n-1)}{n!} = O^* \left( \frac{1}{n^{1-p}} \right) \quad (n \rightarrow \infty)$$

**1.8 Order Estimate (2):**  $\binom{m}{n}$

The binomial coefficient  $\binom{m}{n}$  ( $m \notin \mathbb{N}$ )

$$\binom{m}{n} = \frac{m(m-1)\cdots(m-n+1)}{n!} = O^* \left( \frac{1}{n^{m+1}} \right)$$

**1.9 Order Estimate (3):**  $\frac{(2n)!!}{(2n-1)!!}$  (Wallis' product)

Wallis's product formula has the following forms

$$\frac{(2n)!!}{(2n-1)!!} \sim \sqrt{\pi n} \quad (n \rightarrow \infty)$$

$$\prod_{n=1}^{\infty} \left( \frac{2n}{2n-1} \cdot \frac{2n}{2n+1} \right) = \frac{\pi}{2}$$

$$\lim_{n \rightarrow \infty} \frac{1}{2n+1} \left( \frac{(2n)!!}{(2n-1)!!} \right)^2 = \frac{\pi}{2}$$

### 1.10 Order Estimate (4): $n!$ (Stirling's formula)

The factorial  $n!$  grows at

$$n! \sim \sqrt{2\pi n} \left( \frac{n}{e} \right)^n \quad (n \rightarrow \infty)$$

### 1.11 Definite Integral (1): $\int_0^{\pi/2} \sin^n x dx$

$$\int_0^{\frac{\pi}{2}} \sin^{2n+1} x dx = \frac{(2n)!!}{(2n+1)!!}$$

$$\int_0^{\frac{\pi}{2}} \sin^{2n} x dx = \frac{\pi}{2} \cdot \frac{(2n-1)!!}{(2n)!!}$$

### 1.12 Abel's transformation

The sum  $\sum_{i=1}^m \alpha_i \beta_i$  can be written as

$$\sum_{i=1}^m \alpha_i \beta_i = \alpha_m B_m - \sum_{i=1}^{m-1} (\alpha_{i+1} - \alpha_i) B_i$$

where

$$B_i = \sum_{k=1}^i \beta_k$$

If the original summation does not start with  $i = 1$ , one can write

$$\sum_{i=n}^m a_i b_i = A_m b_m - A_{n-1} b_n + \sum_{i=n}^{m-1} A_i (b_i - b_{i+1})$$

## 2 Inequalities

### 2.1 Bernoulli's Inequality

**Bernoulli's Inequality** For  $x > -1$ ,  $n \in \mathbb{N}^*$ ,

$$(1+x)^n \geq 1+nx$$

and

$$(1+x)^n = 1+nx \iff n=1 \text{ or } x=0$$

**Extensions of Bernoulli's Inequality**

$$x^\alpha - \alpha x + \alpha - 1 \leq 0 \quad \text{when } 0 < \alpha < 1$$

$$x^\alpha - \alpha x + \alpha - 1 \geq 0 \quad \text{when } \alpha < 0 \text{ or } 1 < \alpha$$

### 2.2 Hölder's Inequality

**Hölder's Inequality (for Sums)** Let  $x_i, y_i \geq 0$ ,  $i = 1, \dots, n$ ,  $\frac{1}{p} + \frac{1}{q} = 1$ . Then

$$\sum_{i=1}^n x_i y_i \leq \left( \sum_{i=1}^n x_i^p \right)^{1/p} \left( \sum_{i=1}^n y_i^q \right)^{1/q}, \quad p > 1$$

$$\sum_{i=1}^n x_i y_i \geq \left( \sum_{i=1}^n x_i^p \right)^{1/p} \left( \sum_{i=1}^n y_i^q \right)^{1/q}, \quad p < 1, p \neq 0$$

**Hölder's Inequality (for Integrals)** Let  $f, g \in \mathcal{R}[a, b]$ ,  $\frac{1}{p} + \frac{1}{q} = 1$ . Then

$$\left| \int_a^b (f \cdot g)(x) dx \right| \leq \left( \int_a^b |f|^p(x) dx \right)^{1/p} \cdot \left( \int_a^b |g|^q(x) dx \right)^{1/q}, \quad p > 1$$

### 2.3 Jensen's Inequality

**Jensen's Inequality** If  $f : (a, b) \rightarrow \mathbb{R}$  is a convex function,  $x_1, \dots, x_n \in (a, b)$ , and  $\alpha_1, \dots, \alpha_n$  are positive numbers such that  $\alpha_1 + \dots + \alpha_n = 1$ , then

$$f(\alpha_1 x_1 + \dots + \alpha_n x_n) \leq \alpha_1 f(x_1) + \dots + \alpha_n f(x_n)$$

**Jensen's Inequality (for Integrals)** If  $f$  is a continuous convex function on  $\mathbb{R}$  and  $\varphi$  an arbitrary continuous function on  $\mathbb{R}$ , then

$$f\left(\frac{1}{c} \int_0^c \varphi(t) dt\right) \leq \frac{1}{c} \int_0^c f(\varphi(t)) dt$$

## 2.4 Minkowski's Inequality

**Minkowski's Inequality (for Sums)** Let  $x_i, y_i \geq 0$ ,  $i = 1, \dots, n$ . Then

$$\begin{aligned} \left( \sum_{i=1}^n (x_i + y_i)^p \right)^{1/p} &\leq \left( \sum_{i=1}^n x_i^p \right)^{1/p} + \left( \sum_{i=1}^n y_i^p \right)^{1/p}, \quad p > 1 \\ \left( \sum_{i=1}^n (x_i + y_i)^p \right)^{1/p} &\geq \left( \sum_{i=1}^n x_i^p \right)^{1/p} + \left( \sum_{i=1}^n y_i^p \right)^{1/p}, \quad p < 1, p \neq 0 \end{aligned}$$

**Minkowski's Inequality (for Integrals)** Let  $f, g \in \mathcal{R}[a, b]$ . Then

$$\begin{aligned} \left( \int_a^b |f + g|^p(x) dx \right)^{1/p} &\leq \left( \int_a^b |f|^p(x) dx \right)^{1/p} + \left( \int_a^b |g|^p(x) dx \right)^{1/p}, \quad p \geq 1 \\ \left( \int_a^b |f + g|^p(x) dx \right)^{1/p} &\geq \left( \int_a^b |f|^p(x) dx \right)^{1/p} + \left( \int_a^b |g|^p(x) dx \right)^{1/p}, \quad 0 < p < 1 \end{aligned}$$

## 2.5 Young's Inequality

**Young's Inequality** If  $a > 0$ ,  $b > 0$ , then

$$\begin{aligned} a^{1/p} b^{1/q} &\leq \frac{1}{p} a + \frac{1}{q} b, \quad p > 1 \\ a^{1/p} b^{1/q} &\geq \frac{1}{p} a + \frac{1}{q} b, \quad p < 1 \text{ and } p \neq 0 \end{aligned}$$

and

$$a^{1/p} b^{1/q} = \frac{1}{p} a + \frac{1}{q} b \iff a = b$$

Or it could be written as

$$xy \leq \frac{1}{p} x^p + \frac{1}{q} y^q$$

for  $x, y \geq 0$ ,  $p, q > 0$ ,  $\frac{1}{p} + \frac{1}{q} = 1$

## 3 Numerical Series

### 3.1 Problems

#### 3.1.1 $\sum a_n$ and $\lim na_n$

1.  $\lim_{n \rightarrow \infty} na_n = a \neq 0 \implies \sum_{n=1}^{\infty} a_n$  diverges.

2. If  $a_1 \geq a_2 \geq \cdots \geq a_n \geq \cdots \geq 0$  and  $\sum_{n=1}^{\infty} a_n$  converges, then  $\lim_{n \rightarrow \infty} na_n = 0$ .

**Note 3.1.** *An analog in integral is*

$$\int_a^{+\infty} f(x)dx \text{ converges and } f(x) \text{ is monotonic} \implies f(x) = o\left(\frac{1}{x}\right)$$

3.  $\lim_{n \rightarrow \infty} na_n$  may not exist for a convergent  $\sum_{n=1}^{\infty} a_n$ . For example,

$$a_n = \begin{cases} \frac{1}{n} & , \quad n = m^2 \\ \frac{1}{n^2} & , \quad n \neq m^2 \end{cases}$$

4.  $\lim_{n \rightarrow \infty} na_n = 0$  does not imply the convergence of  $\sum_{n=1}^{\infty} a_n$ . For example,

$$a_n = \frac{1}{n \ln n}$$

### 3.1.2 $\sum a_n$ , $\sum a_n^2$ and $\sum a_n^3$

1. If  $a_n \geq 0$  and  $\sum_{n=1}^{\infty} a_n$  converges, then  $\sum_{n=1}^{\infty} a_n^2$  converges too.

**Note 3.2.** *The converse is untrue. An example is  $a_n = \frac{1}{n}$ .*

2. The convergence of  $\sum_{n=1}^{\infty} a_n$  does not imply that of  $\sum_{n=1}^{\infty} a_n^3$ , for example,

$$a_n = \frac{1}{\sqrt[3]{n}} \cos \frac{2\pi}{3}n$$

### 3.1.3 $\sum a_n$ and $\sum(a_n + a_{n+1})$

The convergence of  $\sum_{n=1}^{\infty} a_n$  implies that of  $\sum_{n=1}^{\infty} (a_n + a_{n+1})$ . The converse is not true, for example

$$a_n = (-1)^n$$

However, the converse is true if  $a_n > 0$ .

### 3.1.4 $\sum a_n$ , $\{na_n\}$ and $\sum(a_n - a_{n+1})$

If  $\{na_n\}$ ,  $\sum_{n=1}^{\infty} n(a_n - a_{n+1})$  converge, then  $\sum_{n=1}^{\infty} a_n$  converges.

### 3.1.5 $\sum a_n$ and $\sum \sqrt{a_n a_{n+1}}$

If  $a_n \geq 0$  and  $\sum_{n=1}^{\infty} a_n$  converges, then  $\sum_{n=1}^{\infty} \sqrt{a_n a_{n+1}}$  converges too. The converse is not true, for example

$$a_n = \begin{cases} \frac{1}{n} & , \quad n = 2k \\ \frac{1}{n^2} & , \quad n = 2k - 1 \end{cases}$$

But the converse is true if  $\{a_n\}$  is monotonically decreasing.

### 3.1.6 $\sum a_n$ and $\sum \frac{a_n^\alpha}{n^\beta}$

1. If  $a_n > 0$  and  $\sum_{n=1}^{\infty} a_n$  converges, and  $\alpha, \beta > 0$  are such that  $\alpha + \beta > 1$ . Then the series

$$\sum_{n=1}^{\infty} \frac{a_n^\alpha}{n^\beta}$$

converges.

**Proof 3.1.** Hölder's inequality.

2. A special case is that

$$a_n > 0, \sum_{n=1}^{\infty} a_n < +\infty \implies \forall \delta > 0, \sum_{n=1}^{\infty} \sqrt{\frac{a_n}{n^{1+\delta}}} < +\infty$$

**Note 3.3.** *The proposition may not be true for  $\delta$ , for example,*

$$\begin{aligned} a_n &= \frac{1}{n(\ln n)^{1+\varepsilon}} \quad (0 < \varepsilon < 1) \\ \implies \sqrt{\frac{a_n}{n}} &= \frac{1}{n(\ln n)^{\frac{1+\varepsilon}{2}}} \quad (0 < \varepsilon < 1) \end{aligned}$$

**Note 3.4.** [E14.2-12]

### 3.1.7 $\sum a_n$ and $\sum \frac{a_n}{1+a_n}, \sum \frac{a_n}{1+n^2 a_n}, \sum \frac{a_n}{1+a_n^2}, \sum \frac{a_n}{1+n a_n}$

Let  $\sum_{n=1}^{\infty} a_n$  be a divergent series with positive terms. Then

1. The series

$$\sum_{n=1}^{\infty} \frac{a_n}{1+a_n}$$

diverges.



**Proof 3.2.** Consider whether  $\limsup_{n \rightarrow \infty} a_n = 0$ . If so, then  $a_n$  is bounded and we can change the denominator to compare with  $\sum_{n=1}^{\infty} a_n$ ; if not, then  $\{a_n\}$  does not tend to 0.

2. The series

$$\sum_{n=1}^{\infty} \frac{a_n}{1 + n^2 a_n}$$

converges.

**Proof 3.3.** Compare with  $\sum_{n=1}^{\infty} \frac{1}{n^2}$

3. The series

$$\sum_{n=1}^{\infty} \frac{a_n}{1 + a_n^2}$$

diverges when  $\{a_n\}$  is bounded. When  $a_n \rightarrow +\infty$ , the series has the same convergence of  $\sum_{n=1}^{\infty} \frac{1}{a_n}$ . Its behavior is uncertain in other situations.

**Note 3.5.** Unlike  $\sum \frac{a_n}{1+a_n}$  where  $\frac{a_n}{1+a_n} \rightarrow 0 \iff a_n \rightarrow 0$ , it may happen that  $\frac{a_n}{1+a_n^2} \rightarrow 0$  but  $a_n \not\rightarrow 0$ .

4. The series

$$\sum_{n=1}^{\infty} \frac{a_n}{1 + n a_n}$$

diverges when  $\{n a_n\}$  is bounded or tends to  $+\infty$ . Its behavior is uncertain in other situations.

**Note 3.6.** [E14.2-11], [P14.2-2]

**3.1.8**  $\sum a_n$  and  $\sum \frac{a_n}{S_n^\alpha}$

Let  $a_n > 0$  and  $S_n = \sum_{k=1}^n a_k$ .

1.  $\alpha > 1 \implies \sum_{n=1}^{\infty} \frac{a_n}{S_n^\alpha}$  converges.

2.  $\alpha \leq 1$  and  $S_n \rightarrow +\infty \implies \sum_{n=1}^{\infty} \frac{a_n}{S_n^\alpha}$  diverges.

**Note 3.7.** [P14.2-3]

**3.1.9**  $\sum a_n \cos nx$  and  $\sum a_n \sin nx$ 

1. If  $a_n \geq 0$  and tends to 0 monotonically, then

$$\sum_{n=1}^{\infty} a_n \cos nx \text{ converges where } x \neq 2k\pi$$

$$\sum_{n=1}^{\infty} a_n \cos nx \text{ has the same convergence as } \sum_{n=1}^{\infty} a_n \text{ when } x = 2k\pi$$

2. If  $a_n \geq 0$ , then

$$\sum_{n=1}^{\infty} a_n \cos nx \text{ converges uniformly on } \mathbb{R} \iff \sum_{n=1}^{\infty} a_n \text{ converges}$$

3. If  $a_n \geq 0$  and tends to 0 monotonically, then

$$\sum_{n=1}^{\infty} a_n \sin nx \text{ converges on } \mathbb{R}$$

4. If  $a_n \geq 0$  and decreases monotonically, then

$$\sum_{n=1}^{\infty} a_n \sin nx \text{ converges uniformly on } \mathbb{R} \iff \lim_{n \rightarrow \infty} na_n = 0$$

**Note 3.8.** [E14.4-6], [E15.2-8], [P15.2-7]

**3.1.10**  $\sum a_n$  and  $\sum \left( \frac{a_{n+1}}{a_n} - 1 \right)$ 

If  $a_n > 0$  and is monotonically increasing, then

$$\sum_{n=1}^{\infty} \left( \frac{a_{n+1}}{a_n} - 1 \right) \text{ converges } \iff \{a_n\} \text{ is bounded}$$

**Note 3.9.** [P14.4-3]

**3.1.11**  $\sum a_n$  and  $\lim_{n \rightarrow \infty} \frac{a_1 + 2a_2 + \cdots + na_n}{n}$ 

If  $\sum_{n=1}^{\infty} a_n$  converges, then

$$\lim_{n \rightarrow \infty} \frac{a_1 + 2a_2 + \cdots + na_n}{n} = 0$$

**Note 3.10.** [E14.4-8]

**3.1.12**  $\sum a_n b_n$  **and**  $\lim(a_1 + \cdots + a_n)b_n$

If  $\{b_n\}$  ( $b_n \geq 0$ ) tends to 0 monotonically and  $\sum_{n=1}^{\infty} a_n b_n$  converges, then

$$\lim_{n \rightarrow \infty} (a_1 + \cdots + a_n)b_n = 0$$

**Note 3.11.** [P14.4-6]

**3.1.13**  $\sum a_n$  **and**  $\lim \frac{a_1 b_1 + a_2 b_2 + \cdots + a_n b_n}{b_n}$

If  $\{b_n\}$  ( $b_n > 0$ ) and tends to  $+\infty$  monotonically and  $\sum_{n=1}^{\infty} a_n$  converges, then

$$\lim_{n \rightarrow \infty} \frac{a_1 b_1 + a_2 b_2 + \cdots + a_n b_n}{b_n} = 0$$

**Note 3.12.** [P14.4-7]

**Note 3.13.** *Go back two problems you will find a special case of this.*

**3.1.14**  $\sum a_n$  **and**  $\sum \frac{a_1 + 2a_2 + \cdots + na_n}{n(n+1)}$

If  $\sum_{n=1}^{\infty} a_n$  converges, then by setting

$$b_n = \frac{a_1 + 2a_2 + \cdots + na_n}{n(n+1)}$$

one can obtain a new series such that

$$\sum_{n=1}^{\infty} b_n = \sum_{n=1}^{\infty} a_n$$

**Note 3.14.** [P14.4-8]

**3.1.15**  $\sum a_n$  **and**  $\lim(a_1 b_n + a_2 b_{n-1} + a_n b_1) = 0$

If  $\sum_{n=1}^{\infty} a_n$  converges absolutely and  $\lim_{n \rightarrow \infty} b_n \rightarrow 0$ , then

$$\lim_{n \rightarrow \infty} (a_1 b_n + a_2 b_{n-1} + a_n b_1) = 0$$

**Note 3.15.** [P14.5-4]

### 3.1.16 Other Problems From Chang & Shi

**P14.1-4** If  $a_n > 0$  and  $\{a_n - a_{n+1}\}$  is a strictly decreasing sequence, then

$$\sum_{n=1}^{\infty} a_n < +\infty \implies \lim_{n \rightarrow \infty} \left( \frac{1}{a_{n+1}} - \frac{1}{a_n} \right) = +\infty$$

**P14.1-5** There exists a constant  $K$  such that

$$\sum_{n=1}^{\infty} \frac{n}{a_1 + a_2 + \cdots + a_n} \leq K \sum_{n=1}^{\infty} \frac{1}{a_n}$$

holds for all sequences  $\{a_n\}$  with positive terms.

**E14.2-4** The following series can be tested by comparison using the Cauchy-Hölder inequality.

**E14.2-6** The series

$$\sum_{n=2}^{\infty} \frac{1}{\ln n!}$$

diverges.

**Proof 3.4.** [Stirling's formula](#)

**E14.2-6** The series

$$\sum_{n=3}^{\infty} \frac{1}{n \ln n \ln \ln n}$$

diverges.

**Proof 3.5.** [Integral test](#). Notice that

$$\int \frac{1}{x \ln x \ln \ln x} dx = \ln \ln \ln x + C$$

**P14.2-1** The series

$$\sum_{n=1}^{\infty} x^{1+\frac{1}{2}+\cdots+\frac{1}{n}}$$

converges for  $0 < x < e^{-1}$  and diverges for  $x \geq e^{-1}$ .

**P14.4-1** Let  $a_n > 0$ . If for  $0 < \alpha < 1$ ,

$$\lim_{n \rightarrow \infty} n^\alpha \left( \frac{a_n}{a_{n+1}} - 1 \right) = \lambda > 0$$

( $\lambda = +\infty$  included), then  $\forall k \in \mathbb{N}$ ,  $\sum_{n=1}^{\infty} n^k a_n$  converges.

**Note 3.16.** *The testing condition resembles that of [E14.4-12], but I don't see much connection here.*

**P14.6-1** The Cauchy product of

$$\sum_{n=1}^{\infty} (-1)^{n-1} \frac{1}{n^\alpha}, \quad \sum_{n=1}^{\infty} (-1)^{n-1} \frac{1}{n^\beta} \quad (\alpha, \beta > 0)$$

converges for  $\alpha + \beta > 1$  and diverges for  $\alpha + \beta \leq 1$ .

**Proof 3.6.** Use Pringsheim's theorem.

## 4 Series of Functions

### 4.1 Problems

#### 4.1.1 Uniform Convergence

**E15.2-4** Let  $u_n(x)$  be monotonic functions on  $[a, b]$ . If  $\sum_{n=1}^{\infty} u_n(a)$ ,  $\sum_{n=1}^{\infty} u_n(b)$  converge absolutely, then  $\sum_{n=1}^{\infty} u_n(x)$  converges absolutely and uniformly on  $[a, b]$ .

**E15.2-7** Let  $u_n(x)$  be continuous functions on  $[a, b]$ . If  $\sum_{n=1}^{\infty} u_n(x)$  converges at every point of  $[a, b)$ , but diverges at  $b$ , then the convergence of  $\sum_{n=1}^{\infty} u_n(x)$  on  $[a, b)$  is not uniform.

**Note 4.1.** *An example is  $\sum_{n=2}^{\infty} \frac{\cos nx}{n \ln n}$ .*

**E15.2-10** Let  $[a, b]$  be a finite closed interval and  $\{f_n\}$  a sequence of functions, then

$$\forall x \in [a, b], \exists \text{ open interval } I_x \ni x, f_n|_{I_x} \Rightarrow f|_{I_x} \implies f_n \Rightarrow f$$

**P15.2-2 (Uniform convergence of product)** Let  $f_n \rightrightarrows f$ ,  $g_n \rightrightarrows g$  on an interval  $I$ . If for each  $n$ ,  $f_n, g_n$  are bounded on  $I$ , then  $f_n g_n \rightrightarrows fg$ .

**Note 4.2.** *In fact, even if they are not required to be uniformly bounded by hypothesis, it can be proved.*

**Note 4.3.** *A counterexample if they are not required to be bounded is*

$$f_n(x) = x(1 + \frac{1}{n}), \quad g_n(x) = \begin{cases} \frac{1}{n} & , \quad x = 0, x \in \mathbb{R} \setminus \mathbb{Q} \\ q + \frac{1}{n} & , \quad x = \frac{p}{q} (q > 0) \end{cases}$$

**P15.2-4 (Bounded derivative series)** Let  $\sum_{n=1}^{\infty} u_n(x)$  be converge on  $[a, b]$ . If

there exists  $M$ , such that for all  $x \in [a, b]$  and  $n \in \mathbb{N}$ ,  $\left| \sum_{k=1}^n u'_k(x) \right| \leq M$ , then

$\sum_{n=1}^{\infty} u_n(x)$  converges uniformly on  $[a, b]$ .

**E15.3-6 (Extension to limit point by uniform convergence)** Let  $E \subset \mathbb{R}$  be a set and  $x_0$  a limit point of  $E$  (it may assume the values  $\pm\infty$ ). If  $\sum_{n=1}^{\infty} u_n(x)$

converges uniformly on  $E$  and  $\lim_{\substack{x \rightarrow x_0 \\ x \in E}} u_n(x) = a_n$ , then  $\sum_{n=1}^{\infty} a_n$  converges and

$$\lim_{\substack{x \rightarrow x_0 \\ x \in E}} \sum_{n=1}^{\infty} u_n(x) = \sum_{n=1}^{\infty} a_n$$

**P15.3-2 (Application of [E15.3-6])** Let the series  $\sum_{n=1}^{\infty} u_n(x)$  satisfy

1.  $\int_a^{+\infty} u_n(x) dx$  converges for all  $n \in \mathbb{N}$ .
2.  $\sum_{n=1}^{\infty} u_n(x)$  converges on  $[a, b]$  for all  $b > a$ .
3.  $\sum_{n=1}^{\infty} \int_a^x u_n(t) dt$  converges uniformly on  $[a, +\infty)$

then  $\int_a^{+\infty} \sum_{n=1}^{\infty} u_n(x) dx$  and  $\sum_{n=1}^{\infty} \int_a^{+\infty} u_n(x) dx$  both converges and are equal to each other

$$\int_a^{+\infty} \sum_{n=1}^{\infty} u_n(x) dx = \sum_{n=1}^{\infty} \int_a^{+\infty} u_n(x) dx$$

**P15.3-3 (Application of [E15.3-6])** Let the series  $\sum_{n=1}^{\infty} u_n(x)$  satisfy

1.  $\sum_{n=1}^{\infty} u_n(x)$  converges to  $f(x)$  on  $(x_0 - \delta, x_0 + \delta)$ .
2.  $u_n(x)$  is differentiable at  $x = x_0$  for all  $n \in \mathbb{N}$ .
3.  $\sum_{n=1}^{\infty} \frac{u_n(x) - u_n(x_0)}{x - x_0}$  converges uniformly on  $(x_0 - \delta, x_0 + \delta) \setminus \{x_0\}$ .

then  $f$  is differentiable at  $x_0$  and

$$f'(x_0) = \sum_{n=1}^{\infty} u'_n(x_0)$$

**P15.3-1 (Bounded convergence and integrability)** Let  $\sum_{n=1}^{\infty} u_n(x)$  converge on  $[a, b]$ . If

$$|S_n(x)| = \left| \sum_{k=1}^n u_k(x) \right| \leq M \quad (a \leq x \leq b, n \in \mathbb{N})$$

then  $\sum_{n=1}^{\infty} u_n(x)$  converges boundedly. Let  $\sum_{n=1}^{\infty} u_n(x)$  converge boundedly on  $[a, b]$ , and converge uniformly on  $[a, c - \delta]$  and  $[c + \delta, b]$  for all  $\delta > 0$  and some fixed  $c$ , then  $u_n(x)$  is integrable on  $[a, b] \implies \sum_{n=1}^{\infty} u_n(x)$  is integrable on  $[a, b]$  and

$$\int_a^b \sum_{n=1}^{\infty} u_n(x) dx = \sum_{n=1}^{\infty} \int_a^b u_n(x) dx$$

#### 4.1.2 Convergence Radius

**E15.4-3 (Sum/product of coefficients)** Let  $\sum_{n=0}^{\infty} a_n x^n$  and  $\sum_{n=0}^{\infty} b_n x^n$  have convergence radii  $R_1$  and  $R_2$ , then

1.  $\sum_{n=0}^{\infty} (a_n + b_n) x^n$  has convergence radius  $R \geq \min(R_1, R_2)$ .
2.  $\sum_{n=0}^{\infty} (a_n b_n) x^n$  has convergence radius  $R \geq R_1 R_2$ .
3. It may happen that the last two inequalities are strict.

**E15.4-6** The convergence radius  $R$  of  $\sum_{n=0}^{\infty} a_n x^n$  satisfies

$$\liminf_{n \rightarrow \infty} \left| \frac{a_n}{a_{n+1}} \right| = l \leq R \leq L = \limsup_{n \rightarrow \infty} \left| \frac{a_n}{a_{n+1}} \right|$$

**P15.4-5 (Limit to the edge)** Let  $\sum_{n=0}^{\infty} a_n x^n$  have convergence radius  $R$  and  $a_n \geq 0$ , then

$$\lim_{x \rightarrow R^-} \sum_{n=0}^{\infty} a_n x^n = \sum_{n=0}^{\infty} a_n R^n$$

### 4.1.3 Other Problems from Chang & Shi

**E15.2-3**  $\sum_{n=1}^{\infty} a_n$  converges  $\implies \sum_{n=1}^{\infty} a_n e^{-nx}$  converges uniformly on  $[0, +\infty)$ .

**E15.2-10**  $\alpha < 1 \iff f_n(x) = x n^{-x} (\ln n)^{\alpha}$  converges uniformly on  $[0, +\infty)$ .

**E15.2-12** Let  $f_1$  be Riemann integrable on  $[a, b]$  and define

$$f_{n+1}(x) = \int_a^x f_n(t) dt$$

, then  $f_n \Rightarrow 0$  on  $[a, b]$ .

**Note 4.4.** *Should I try successive approximation of Picard on this?*

**E15.2-13**  $\alpha > 2 \implies \sum_{n=1}^{\infty} x^{\alpha} e^{-nx^2}$  converges uniformly on  $[0, +\infty)$ .

**P15.2-1**  $\sum_{n=1}^{\infty} \frac{nx}{(1+x)(1+2x)\cdots(1+nx)}$  converges nonuniformly on  $[0, \delta]$  and uniformly on  $[\delta, +\infty)$  for all  $\delta > 0$ .

**P15.2-5** Let  $f \in C^2$  in some neighborhood of  $x = 0$  and  $f(0) = 0$ ,  $0 < f'(0) < 1$ .

Denote  $\underbrace{f \circ f \circ \cdots \circ f}_n$  by  $f_n$ . The series  $\sum_{n=1}^{\infty} f_n(x)$  converges uniformly in a neighborhood of 0.

**P15.2-6**  $\sum_{n=1}^{\infty} \frac{x^n}{1+x+x^2+\cdots+x^{2n-1}} \cos nx$  converges uniformly on  $[0, 1]$



**P15.3-4** Let  $\{a_n\}$  be a sequence in  $(0, 1)$  and  $a_i \neq a_j$  for all  $i \neq j$ , then

$$f(x) = \sum_{n=1}^{\infty} \frac{|x - a_n|}{2^n}$$

is continuous on  $(0, 1)$ , and is nondifferentiable at each  $x = a_n$  and differentiable everywhere else.

**P15.3-5** Let  $f(x) = \sum_{n=0}^{\infty} \frac{1}{x+2^n}$  ( $0 \leq x < +\infty$ ), then

1.  $f$  is continuous on  $[0, +\infty)$ .
2.  $\lim_{x \rightarrow +\infty} f(x) = 0$
3. For all  $x \in (0, +\infty)$ ,

$$0 < f(x) - \frac{\ln(1+x)}{x \ln 2} < \frac{1}{1+x}$$

**P15.3-6**

$$\sum_{n=0}^{\infty} \frac{(n!)^2 2^{n+1}}{(2n+1)!} = \pi$$

**P15.3-7** Define a function  $\varphi$  as follows:

$$\begin{aligned} \varphi(x) &= x(1-x) \quad (0 \leq x \leq 1) \\ \varphi(-x) &= -\varphi(x) \\ \varphi(x+2) &= \varphi(x) \end{aligned}$$

then

$$f(x) = \sum_{n=0}^{\infty} \frac{\varphi(n!x)}{(n!)^2}$$

assumes rational values at rational points and irrational values at irrational points.